precondition normalization:   well-formedness   applying formula maps to dnf_list

Precondition_Normalization.thy
@@ -3,24 +3,26 @@ imports "AI_Planning_Languages_Semantics.PDDL_STRIPS_Semantics"
     PDDL_Sema_Supplement Utils String_Shenanigans DNF
 begin
 
-definition "n_clauses ac \<equiv> length (dnf_list (ast_action_schema.precondition ac))"
+definition "n_clauses ac \<equiv> length (dnf_list (ac_pre ac))"
+abbreviation "max_length' xs \<equiv> Max (length ` set xs)"
 
 context ast_domain begin
 
 definition "max_n_clauses \<equiv> Max (set (map n_clauses (actions D)))"
-definition "prefix_padding \<equiv> max_length (distinct_strings max_n_clauses) + 1"
+definition "prefix_padding \<equiv> max_length' (distinct_strings max_n_clauses) + 1"
 
 fun (in -) set_n_pre :: " ast_action_schema \<Rightarrow> string \<Rightarrow> term atom formula \<Rightarrow> ast_action_schema" where
   "set_n_pre (Action_Schema _ params _ eff) n pre
   = Action_Schema n params pre eff"
 
-definition "split_ac_names ac n \<equiv>
-  map (\<lambda>prefix. pad prefix_padding prefix @ ac_name ac) (distinct_strings n)"
+definition "split_ac_names ac \<equiv>
+  map (\<lambda>prefix. pad prefix_padding prefix @ ac_name ac)
+    (distinct_strings (n_clauses ac))"
 
 definition split_ac :: "ast_action_schema \<Rightarrow> ast_action_schema list" where
   "split_ac ac =
     (let clauses = dnf_list (ac_pre ac) in
-    map2 (set_n_pre ac) (split_ac_names ac (length clauses)) clauses)"
+    map2 (set_n_pre ac) (split_ac_names ac) clauses)"
 
 definition "split_acs \<equiv> concat (map split_ac (actions D))"
 
@@ -90,19 +92,13 @@ lemma set_n_pre_sel [simp]:
   "ac_eff (set_n_pre ac n pre) = ac_eff ac"
   using set_n_pre_alt by simp_all
 
-thm ast_domain.split_ac_def
-
-lemma
-  "i < length as \<Longrightarrow> i < length bs \<Longrightarrow> map2 f as bs ! i = f (as!i) (bs!i)"
-  by simp
-
-lemma (in ast_domain)
-  assumes "i < length (dnf_list (ac_pre ac))"
-  shows "split_ac ac ! i =
-    set_n_pre ac
-    ((\<lambda>prefix. pad prefix_padding prefix @ ac_name ac) (distinct_strings (length (dnf_list (ac_pre ac))) ! i))
-    (dnf_list (ac_pre ac) ! i)"
-  using assms unfolding split_ac_def split_ac_names_def set_n_pre_alt Let_def sorry
+lemma (in -) set_n_pre_mapsel:
+  assumes "length ns = length pres"
+  shows
+    "map ac_name (map2 (set_n_pre ac) ns pres) = ns"
+    (*"map ac_params (map2 (set_n_pre ac) ns pres) = replicate (n_clauses ac) (ac_params ac)" *)
+    "map ac_pre (map2 (set_n_pre ac) ns pres) = pres"
+using assms by (induction ns pres rule: list_induct2) simp_all
 
 lemma (in ast_domain) split_dom_sel [simp]:
   "types D4 = types D"
@@ -118,26 +114,405 @@ lemma (in ast_problem) split_prob_sel [simp]:
   "goal P4 = goal P"
   using split_prob_def by simp_all
 
+text \<open> Action splitting properties \<close>
+lemma (in ast_domain) split_ac_len:
+  "length (split_ac ac) = length (dnf_list (ac_pre ac))"
+  "length (split_ac_names ac) = length (dnf_list (ac_pre ac))"
+  unfolding split_ac_def split_ac_names_def n_clauses_def by simp_all
+
+lemma (in ast_domain) split_ac_nth:
+  assumes "i < length (dnf_list (ac_pre ac))"
+  shows "split_ac ac ! i =
+    Action_Schema
+      (pad prefix_padding (unique_string i) @ ac_name ac)
+      (ac_params ac)
+      (dnf_list (ac_pre ac) ! i)
+      (ac_eff ac)"
+  using assms unfolding split_ac_def split_ac_names_def n_clauses_def
+  by (cases ac) simp
+
+lemma (in ast_domain4) p_ac:
+  "ac' \<in> set (actions D4) \<longleftrightarrow> (\<exists>ac \<in> set (actions D). ac' \<in> set (split_ac ac))"
+  unfolding split_dom_sel split_acs_def by simp
+
+lemma (in ast_domain) split_pres: "map ac_pre (split_ac a) = dnf_list (ac_pre a)"
+    unfolding split_ac_def Let_def apply (rule set_n_pre_mapsel)
+    unfolding split_ac_names_def n_clauses_def by simp
+
+(* "ac_params a' = ac_params a" "ac_eff a' = ac_eff a" if "a' \<in> set (split_ac a)" *)
+
+
+lemma (in ast_domain) split_ac_sel:
+  assumes "a' \<in> set (split_ac a)"
+  shows
+    "\<exists>i < length (split_ac a). ac_name a' = pad prefix_padding (unique_string i) @ ac_name a"
+    "ac_params a' = ac_params a"
+    "ac_pre a' \<in> set (dnf_list (ac_pre a))"
+    "ac_eff a' = ac_eff a"
+proof -
+  from assms show "ac_params a' = ac_params a" "ac_eff a' = ac_eff a"
+    unfolding split_ac_def Let_def by auto
+  from assms obtain i where i: "i < length (split_ac a)" "a' = split_ac a ! i"
+    using in_set_conv_nth by metis
+  from i show "ac_pre a' \<in> set (dnf_list (ac_pre a))"
+    using split_ac_nth split_ac_len(1) by simp
+  from i show "\<exists>i < length (split_ac a). ac_name a' = pad prefix_padding (unique_string i) @ ac_name a"
+    using split_ac_nth split_ac_len(1) by auto
+qed
 
 subsection \<open> Output format \<close>
 
-context ast_problem4 begin
-thm precond_normed_dom_def
-(* \<forall>ac \<in> set (actions D). is_conj (ac_pre ac) *)
-
-thm split_ac_def
-lemma prec_normed_ac:
+lemma (in ast_problem4) prec_normed_ac:
   "\<forall>ac' \<in> set (split_ac ac). is_conj (ac_pre ac')"
-proof -
-  have "\<forall>c \<in> set (dnf_list (ac_pre ac)). is_conj c"
-    using dnf_list_conjs by auto
-  have "\<forall>ac' \<in> set (split_ac ac). ac_pre ac \<in>
-    set (dnf_list (ac_pre ac))" unfolding split_ac_def Let_def sorry
-  thus ?thesis
-    unfolding split_ac_def Let_def sorry
-qed
+  using split_ac_sel(3) dnf_list_conjs by auto
+
+subsection \<open> Well-formedness \<close>
+
+context ast_domain4 begin
+
+lemma p_wf_type: "d4.wf_type = wf_type"
+  apply (rule ext)
+  subgoal for x
+    by (cases x; simp)
+  done
+
+lemma p_wf_pred_decl: "d4.wf_predicate_decl = wf_predicate_decl"
+  apply (rule ext)
+  subgoal for x                                      
+    apply (cases x; simp) using p_wf_type by simp
+  done
+
+lemma p_constT: "d4.constT = constT"
+  unfolding ast_domain.constT_def by simp
+
+lemma (in ast_problem4) p_objT: "p4.objT = objT"
+  unfolding ast_problem.objT_def using p_constT by simp
+
+lemma p_sig: "d4.sig = sig"
+  unfolding ast_domain.sig_def by simp
+
+lemma p_subtype_rel: "d4.subtype_rel = subtype_rel"
+  unfolding ast_domain.subtype_rel_def by simp
+
+lemma p_of_type: "d4.of_type = of_type"
+  unfolding ast_domain.of_type_def using p_subtype_rel by simp
+
+lemma p_is_of_type: "d4.is_of_type = is_of_type"
+  unfolding ast_domain.is_of_type_def using p_of_type by metis
+
+lemma p_wf_atom: "d4.wf_atom = wf_atom"
+  apply (rule ext; rule ext)
+  subgoal for tyt x
+    apply (cases x; simp)
+    using split_dom_sel(1-2) p_sig p_is_of_type by metis
+  done
+
+lemma p_wf_fmla: "d4.wf_fmla = wf_fmla"
+  unfolding ast_domain.wf_fmla_alt using p_wf_atom by metis
+
+lemma p_wf_eff: "d4.wf_effect = wf_effect"
+  unfolding ast_domain.wf_effect_alt ast_domain.wf_fmla_atom_alt
+  using p_wf_fmla by metis
+
+lemma (in ast_problem4) p_wf_wm: "p4.wf_world_model = wf_world_model"
+  unfolding ast_problem.wf_world_model_def ast_domain.wf_fmla_atom_alt
+  using p_wf_fmla p_objT split_prob_sel(1) by metis
 
 end
+context wf_ast_domain4 begin
+
+(* generated action IDs are distinct *)
+(* TODO: simplify; combine with split_ac_sel *)
+
+lemma (in ast_domain) split_names_prefix_length:
+  assumes "ac \<in> set (actions D)" "n \<in> set (split_ac_names ac)"
+  shows "\<exists>p. length p = prefix_padding \<and> n = p @ ac_name ac"
+proof -
+  from assms(2)[unfolded split_ac_names_def] obtain p where
+    pin: "p \<in> set (distinct_strings (n_clauses ac))" and
+    n: "n = pad prefix_padding p @ ac_name ac"
+    by auto
+
+  have "n_clauses ac \<le> max_n_clauses"
+    using max_n_clauses_def assms(1) by simp
+  hence "prefix (distinct_strings (n_clauses ac)) (distinct_strings (max_n_clauses))"
+    using distinct_strings_prefix by (metis le_Suc_ex)
+  hence "set (distinct_strings (n_clauses ac)) \<subseteq> set (distinct_strings (max_n_clauses))"
+    using set_mono_prefix by auto
+  hence "length p \<le> prefix_padding"
+    unfolding prefix_padding_def
+    apply (intro trans_le_add1)
+    using pin by auto (* I'm relieved auto solves that *)
+  hence "length (pad prefix_padding p) = prefix_padding"
+    using pad_length(1) by auto
+  thus ?thesis using n by simp
+qed
+
+lemma (in ast_domain) split_names_distinct:
+  shows "distinct (split_ac_names ac)"
+proof -
+  have "split_ac_names ac =
+    map (\<lambda>p. p @ ac_name ac) (map (pad prefix_padding) (distinct_strings (n_clauses ac)))"
+    unfolding split_ac_names_def by simp
+  thus ?thesis using distinct_strings_padded append_r_distinct by metis
+qed
+
+lemma (in wf_ast_domain) split_names_disjoint:
+  assumes "ac \<in> set (actions D)" "ac' \<in> set (actions D)" "ac_name ac \<noteq> ac_name ac'"
+  shows "set (split_ac_names ac) \<inter> set (split_ac_names ac') = {}"
+  apply (unfold disjoint_iff_not_equal)
+  using assms split_names_prefix_length
+  using append_eq_append_conv by metis
+
+(* TODO generalize to Utils:
+  distinct xs \<Longrightarrow> x \<noteq> y; \<in> set xs \<longrightarrow> f x \<inter> f y = {} \<Longrightarrow> distinct (removeAll ... *)
+lemma (in wf_ast_domain) split_names_dist_nonempty:
+  "distinct (removeAll [] (map split_ac_names (actions D)))"
+proof -
+  have "distinct (removeAll [] (map split_ac_names as))"
+    if "distinct (map ac_name as)" "set as \<subseteq> set (actions D)" for as
+    using that
+  proof (induction as)
+    case (Cons a as)
+    thus ?case proof (cases "split_ac_names a = []")
+      case False
+
+      from Cons.prems have ain: "\<forall>a' \<in> set as. a' \<in> set (actions D)" "a \<in> set (actions D)" by auto
+
+      from Cons that have "\<forall>n \<in> set (map ac_name as). ac_name a \<noteq> n" by auto
+      hence "\<forall>a' \<in> set as. ac_name a' \<noteq> ac_name a" by auto
+      with ain have "\<forall>a' \<in> set as. set (split_ac_names a) \<inter> set (split_ac_names a') = {}"
+        using split_names_disjoint by blast
+      hence "\<forall>s \<in> set (removeAll [] (map split_ac_names as)). set (split_ac_names a) \<inter> set s = {}" by auto
+      with False have "split_ac_names a \<notin> set (removeAll [] (map split_ac_names as))" by blast
+      then show ?thesis using False Cons by simp
+    qed (simp add: Cons)
+    
+  qed simp
+  thus ?thesis using wf_D(6) by simp
+qed
+
+lemma (in wf_ast_domain) split_names_disjoint2:
+  assumes "xs \<in> set (map split_ac_names (actions D))"
+          "ys \<in> set (map split_ac_names (actions D))"
+          "xs \<noteq> ys"
+        shows "set xs \<inter> set ys = {}"
+proof -
+  from assms obtain x y where
+    xy: "xs = split_ac_names x"  "x \<in> set (actions D)"
+        "ys = split_ac_names y"  "y \<in> set (actions D)" by auto
+  hence "x \<noteq> y" using assms(3) by blast
+  hence "ac_name x \<noteq> ac_name y" using wf_D xy
+    by (meson distinct_map_eq)
+  thus ?thesis
+    using split_names_disjoint xy by simp
+qed
+
+lemma (in ast_domain4) p_ac_names:
+  "map ac_name (actions D4) = concat (map split_ac_names (actions D))"
+proof -
+  have l: "length (split_ac_names ac) = length (dnf_list (ac_pre ac))" for ac
+    unfolding split_ac_names_def n_clauses_def by simp
+
+  have "map ac_name (actions D4) = concat
+      (map (map ac_name) (map split_ac (actions D)))"
+    unfolding split_dom_sel split_acs_def
+    using map_concat by metis
+  also have "... = concat
+      (map (map ac_name \<circ> split_ac) (actions D))" by simp
+  also have "... = concat (map split_ac_names (actions D))"
+    unfolding split_ac_def comp_def
+    using set_n_pre_mapsel(1) l by simp
+  finally show ?thesis .
+qed
+
+lemma split_ac_names_dist:
+  "distinct (map ac_name (actions D4))"
+  unfolding p_ac_names distinct_concat_iff
+  using split_names_dist_nonempty split_names_distinct split_names_disjoint2 by auto
+
+(* action well-formedness *)
+
+lemma p_actions_wf: "list_all1 d4.wf_action_schema (actions D4)"
+proof
+  fix a' assume assm: "a' \<in> set (actions D4)"
+  then obtain a where a: "a \<in> set (actions D)" "a' \<in> set (split_ac a)" using p_ac by auto
+  hence "atoms (ac_pre a') \<subseteq> atoms (ac_pre a)" using split_ac_sel(3) dnf_list_atoms by metis
+  hence fmla_wf: "d4.wf_fmla tyt (ac_pre a')" if "wf_fmla tyt (ac_pre a)" for tyt
+    unfolding p_wf_fmla
+    using that ast_domain.wf_fmla_alt p_wf_fmla by blast
+
+  have "d4.wf_action_schema a'" if "wf_action_schema a"
+    using that unfolding ast_domain.wf_action_schema_alt
+    using a(2) split_ac_sel p_constT fmla_wf p_wf_eff by metis
+
+  thus "d4.wf_action_schema a'" using a(1) wf_D by simp
+qed
+
+theorem (in wf_ast_domain4) p_dom_wf: "d4.wf_domain"
+  unfolding d4.wf_domain_def split_dom_sel
+  unfolding p_wf_type p_wf_pred_decl
+  using wf_D split_ac_names_dist p_actions_wf ast_domain.wf_types_def by simp_all
+
+theorem (in wf_ast_problem4) p_prob_wf: "p4.wf_problem"
+  unfolding p4.wf_problem_def split_prob_sel
+  unfolding p_wf_type p_wf_wm p_wf_fmla p_objT
+  using wf_P p_dom_wf by simp_all
+
+end
+
+subsection \<open> Semantics \<close>
+
+context wf_ast_problem4 begin
+
+lemma dnf_list_cw:
+  assumes "wm_basic M"
+  shows "M \<^sup>c\<TTurnstile>\<^sub>= F \<longleftrightarrow> (\<exists>c\<in>set (dnf_list F). M \<^sup>c\<TTurnstile>\<^sub>= c)"
+  using assms valuation_iff_close_world dnf_list_semantics by blast
+
+text \<open> Applying a map to dnf_list \<close>
+
+lemma (in -) neg_of_lit_map: "map_formula m (neg_of_lit l) = neg_of_lit (map_literal m l)"
+  by (cases l) simp_all
+
+lemma (in -) neg_conj_of_clause_map: "map_formula m (neg_conj_of_clause c)
+  = neg_conj_of_clause (map (map_literal m) c)"
+  unfolding neg_conj_of_clause_def
+  apply (induction c) apply simp using neg_of_lit_map by auto
+  
+lemma (in -) neg_conj_of_clause_map2: "map ((map_formula m) \<circ> neg_conj_of_clause) D
+  = map neg_conj_of_clause (map (map (map_literal m)) D)"
+  using neg_conj_of_clause_map by auto
+
+lemma (in -) nnf_map: "map_formula m (nnf F) = nnf (map_formula m F)"
+  by (induction F rule: nnf.induct) auto
+
+(* there's gotta be some easier way to prove this *)
+(* this works for all g where "f (g x y) = g (f x) (f y)" *)
+lemma (in -) append_prod_map:
+  "map (map f) [x @ y. x \<leftarrow> xs, y \<leftarrow> ys] = [x @ y. x \<leftarrow> map (map f) xs, y \<leftarrow> map (map f) ys]"
+proof -
+  define m where "m = map f"
+  have aux: "map (\<lambda>x. f (g x)) xs = map f (map g xs)" for f g xs by simp
+
+  (* "map f [x @ y. x \<leftarrow> xs, y \<leftarrow> ys] = map f (concat (map (\<lambda>x. map ((@) x) ys) xs))" *)
+  have "map m [x @ y. x \<leftarrow> xs, y \<leftarrow> ys] = (concat (map (map m) (map (\<lambda>x. map ((@) x) ys) xs)))"
+    using map_concat by blast
+  also have "... = concat (map ((map m) \<circ> (\<lambda>x. map ((@) x) ys)) xs)" by simp
+  also have "... = concat (map (\<lambda>x. map m (map ((@) x) ys)) xs)" by (meson comp_apply)
+  also have "... = concat (map (\<lambda>x. map (m \<circ> ((@) x)) ys) xs)" by simp
+  also have "... = concat (map (\<lambda>x. map (\<lambda>y. m (x @ y)) ys) xs)"
+    by (metis fun_comp_eq_conv[of m])
+  also have "... = concat (map (\<lambda>x. map (\<lambda>y. m x @ m y) ys) xs)"
+    unfolding m_def by simp
+  also have "... = concat (map (\<lambda>x. map (\<lambda>y. m x @ y) (map m ys)) xs)"
+    using aux by metis
+  also have "... = concat (map (\<lambda>x. map (\<lambda>y. x @ y) (map m ys)) (map m xs))"
+    using aux[of "(\<lambda>x. map (\<lambda>y. x @ y) (map m ys))"] by metis
+  finally show ?thesis unfolding m_def by simp
+qed
+
+lemma (in -) cnf_lists_map:
+  assumes "is_nnf F"
+  shows "map (map (map_literal m)) (cnf_lists F) = cnf_lists (map_formula m F)"
+  using assms proof (induction F rule: cnf_lists.induct)
+  case (6 F G)
+    define mp where "mp = (map (map_literal m))"
+    have "map mp (cnf_lists (F \<^bold>\<or> G)) = map mp [f @ g. f \<leftarrow> (cnf_lists F), g \<leftarrow> (cnf_lists G)]" by simp
+    also have "... = [f @ g. f \<leftarrow> map mp (cnf_lists F), g \<leftarrow> map mp (cnf_lists G)]"
+      unfolding mp_def using append_prod_map by auto
+    also have "... = [f @ g. f \<leftarrow> cnf_lists (map_formula m F), g \<leftarrow> cnf_lists (map_formula m G)]"
+      using 6 unfolding mp_def by fastforce
+    finally show ?case unfolding mp_def by simp
+qed simp_all
+
+lemma dnf_list_map: "map (map_formula m) (dnf_list F) = dnf_list (map_formula m F)"
+proof -
+  have "map (map_formula m) (dnf_list F)
+    = map (map_formula m) (map neg_conj_of_clause (cnf_lists (nnf (\<^bold>\<not> F))))"
+    unfolding dnf_list_def ..
+  also have "... = map ((map_formula m) \<circ> neg_conj_of_clause) (cnf_lists (nnf (\<^bold>\<not> F)))"
+    by simp
+  also have "... = map neg_conj_of_clause (map (map (map_literal m)) (cnf_lists (nnf (\<^bold>\<not> F))))"
+    using neg_conj_of_clause_map by auto
+  also have "... = map neg_conj_of_clause (cnf_lists (map_formula m (nnf (\<^bold>\<not> F))))"
+    using cnf_lists_map by (metis is_nnf_nnf)
+  also have "... = map neg_conj_of_clause (cnf_lists (nnf (\<^bold>\<not> (map_formula m F))))"
+    using nnf_map formula.map(3) by metis
+  finally show ?thesis unfolding dnf_list_def by simp
+qed
+
+(* end map *)
+
+term ac_tsubst
+term resolve_instantiate
+term instantiate_action_schema
+term map_atom_fmla
+
+lemma
+  "A \<Turnstile> ac_pre a \<longleftrightarrow> (\<exists>a' \<in> set (split_ac a). A \<Turnstile> ac_pre a')"
+proof -
+  let ?dnf = "dnf_list (ac_pre a)"
+  have "A \<Turnstile> ac_pre a \<longleftrightarrow> (\<exists>p' \<in> set ?dnf. A \<Turnstile> p')"
+    using dnf_list_semantics by blast
+  also have "... \<longleftrightarrow> (\<exists>i < length ?dnf. A \<Turnstile> ?dnf ! i)"
+    using in_set_conv_nth by metis
+  also have "... \<longleftrightarrow> (\<exists>i < length ?dnf. A \<Turnstile> ac_pre (split_ac a ! i))"
+    using split_ac_nth by auto
+  also have "... \<longleftrightarrow> (\<exists>a' \<in> set (split_ac a). A \<Turnstile> ac_pre a')"
+    using in_set_conv_nth split_ac_len by metis
+  finally show ?thesis by simp
+qed
+
+lemma
+  assumes "wm_basic M"
+  shows "M \<^sup>c\<TTurnstile>\<^sub>= precondition (instantiate_action_schema a args) \<longleftrightarrow>
+    (\<exists>a' \<in> set (split_ac a). M \<^sup>c\<TTurnstile>\<^sub>= precondition (instantiate_action_schema a' args))"
+proof -
+  oops  
+
+lemma "a \<in> set (actions D) \<Longrightarrow> \<exists>n. resolve_action_schema n = Some a"
+  by (simp add: res_aux)
+
+
+(* TODO move to Utils *)
+(* kind of useless, saves a a line or two sometimes *)
+lemma (in -) list_induct_n:
+  assumes "length xs = n" "P [] 0"
+  "\<And>x xs n. length xs = n \<Longrightarrow>
+  P xs n \<Longrightarrow> P (x # xs) (Suc n)" shows "P xs n"
+using assms proof (induction xs arbitrary: n)
+  case (Cons x xs n)
+  thus ?case by (cases n) simp_all
+qed simp
+
+(* TODO move to Utils *)
+lemma (in -) drop_prefix:
+  assumes "length xs = n" shows "drop n (xs @ ys) = ys"
+  by (induction rule: list_induct_n[OF assms]) simp_all
+
+lemma restore_split_ac:
+  assumes "a \<in> set (actions D)" "a' \<in> set (split_ac a)"
+  shows "drop prefix_padding (ac_name a') = ac_name a"
+proof -
+  (* TODO simplify the start *)
+  from assms obtain i where i: "split_ac a ! i = a'" "i < length (split_ac a)"
+    by (meson in_set_conv_nth)
+  hence "ac_name a' \<in> set (map ac_name (split_ac a))" by auto
+  hence "ac_name a' \<in> set (split_ac_names a)"
+    unfolding split_ac_def
+    using split_ac_len set_n_pre_mapsel by metis
+  thus ?thesis
+    using assms split_names_prefix_length drop_prefix by metis
+qed
+
+thm restore_pa_split.simps
+(*(drop prefix_padding ?n)*)
+thm split_ac_nth
+thm dnf_list_semantics
+
+end
+
 
 subsection \<open> Code Setup \<close>
 
