String_Shenanigans.thy
@@ -1,5 +1,5 @@
 theory String_Shenanigans
-imports Main "Show.Show_Instances"
+imports Main "Show.Show_Instances" "HOL-Library.Sublist"
 begin
 
 fun max_length :: "'a list list \<Rightarrow> nat" where
@@ -36,14 +36,76 @@ lemma dist_prefix: "distinct xs \<Longrightarrow> distinct (map ((@) (safe_prefi
 definition pad :: "nat \<Rightarrow> string \<Rightarrow> string" where
   "pad n s \<equiv> s @ replicate (n - length s) (CHR ''_'')"
 
-definition pad_l :: "nat \<Rightarrow> string \<Rightarrow> string" where
-  "pad_l n s \<equiv> replicate (n - length s) (CHR ''_'') @ s"
+definition padl :: "nat \<Rightarrow> string \<Rightarrow> string" where
+  "padl n s \<equiv> replicate (n - length s) (CHR ''_'') @ s"
 
 lemma pad_length:
   "n \<ge> length s \<Longrightarrow> length (pad n s) = n"
   "length (pad n s) \<ge> n"
   "length (pad n s) \<ge> length s"
   unfolding pad_def by simp_all
+
+lemma padl_length:
+  "n \<ge> length s \<Longrightarrow> length (padl n s) = n"
+  "length (padl n s) \<ge> n"
+  "length (padl n s) \<ge> length s"
+  unfolding padl_def by simp_all
+
+lemma count_replicate: "count_list (replicate n x) x = n"
+  by (induction n) simp_all
+
+lemma count_pad:
+  assumes "CHR ''_'' \<notin> set xs"
+  shows "count_list (pad n xs) (CHR ''_'') = n - length xs"
+  unfolding pad_def using assms count_replicate by fastforce
+
+lemma count_padl:
+  assumes "CHR ''_'' \<notin> set xs"
+  shows "count_list (padl n xs) (CHR ''_'') = n - length xs"
+  unfolding padl_def using assms count_replicate by fastforce
+
+(* Omitting "n \<ge> length xs" "n \<ge> length ys" from assumptions because it's unnecessary*)
+lemma pad_neq:
+  assumes "(CHR ''_'') \<notin> set xs" "CHR ''_'' \<notin> set ys" "xs \<noteq> ys"
+  shows "pad n xs \<noteq> pad n ys"
+proof (cases "length xs = length ys")
+  case False
+  from False consider
+      (neq) "n - length xs \<noteq> n - length ys" |
+      (zero) "n - length xs = 0 \<and> n - length ys = 0"
+    by linarith
+  then show ?thesis
+  proof (cases)
+    case neq
+    moreover have "count_list (pad n ys) (CHR ''_'') = n - length ys" using assms(2) count_pad by simp
+    moreover have "count_list (pad n xs) (CHR ''_'') = n - length xs" using assms(1) count_pad by simp
+    ultimately show ?thesis by metis
+  next
+    case zero
+    thus ?thesis using False pad_def by auto
+  qed
+qed (simp add: pad_def assms(3))
+
+lemma padl_neq:
+  assumes "(CHR ''_'') \<notin> set xs" "CHR ''_'' \<notin> set ys" "xs \<noteq> ys"
+  shows "padl n xs \<noteq> padl n ys"
+proof (cases "length xs = length ys")
+  case False
+  from False consider
+      (neq) "n - length xs \<noteq> n - length ys" |
+      (zero) "n - length xs = 0 \<and> n - length ys = 0"
+    by linarith
+  then show ?thesis
+  proof (cases)
+    case neq
+    moreover have "count_list (padl n ys) (CHR ''_'') = n - length ys" using assms(2) count_padl by simp
+    moreover have "count_list (padl n xs) (CHR ''_'') = n - length xs" using assms(1) count_padl by simp
+    ultimately show ?thesis by metis
+  next
+    case zero
+    thus ?thesis using False padl_def by auto
+  qed
+qed (simp add: padl_def assms(3))
 
 definition make_unique :: "string list \<Rightarrow> string \<Rightarrow> string" where
   "make_unique ss s \<equiv> pad (max_length ss + 1) s"
@@ -60,6 +122,9 @@ qed
 
 definition pad_strings :: "string list \<Rightarrow> string list" where
   "pad_strings ss \<equiv> map (pad (max_length ss + 1)) ss"
+
+
+(* nat upto *)
 
 fun nat_upto_help :: "nat \<Rightarrow> nat list \<Rightarrow> nat list" where
   "nat_upto_help 0 build = 0 # build" |
@@ -102,6 +167,19 @@ qed simp
 lemma nat_upto_nth [simp]: assumes "i \<le> n" shows "nat_upto n ! i = i"
   using assms nat_upto_help_nth nat_upto_def by simp
 
+lemma nat_upto_snoc: "nat_upto (Suc n) = nat_upto n @ [Suc n]"
+  unfolding nat_upto_def
+  apply simp using nat_upto_help_aux
+  by (metis eq_Nil_appendI)
+
+
+lemma nat_upto_prefix: "prefix (nat_upto n) (nat_upto (n+k))"
+  apply (induction k)
+   apply simp
+  apply (subst add_Suc_right)
+  apply (subst nat_upto_snoc)
+  using prefix_def by auto
+
 lemma nat_upto_distinct: "distinct (nat_upto n)"
 proof -
   have "nat_upto n ! i \<noteq> nat_upto n ! j" if "i \<noteq> j" "i \<le> n" "j \<le> n" for i j
@@ -113,8 +191,12 @@ qed
 definition "unique_string (i::nat) \<equiv> show i"
 definition "distinct_strings n \<equiv> map unique_string (case n of 0 \<Rightarrow> [] | Suc m \<Rightarrow> nat_upto m)"
 
+(* TODO: https://isabelle.zulipchat.com/#narrow/channel/238552-Beginner-Questions/topic/String.20inequality.20with.20show/near/500270718*)
 lemma show_nat_inj: fixes a :: nat and b :: nat assumes "a \<noteq> b" shows "show a \<noteq> show b"
   using assms sorry
+
+(* TODO *)
+lemma notin_show_nat: "CHR ''_'' \<notin> set (show (n::nat))" sorry
 
 lemma unique_str_bij:
   "i \<noteq> j \<longleftrightarrow> unique_string i \<noteq> unique_string j"
@@ -131,6 +213,32 @@ lemma distinct_strings_nth [simp]:
 lemma distinct_strings_dist:
   "distinct (distinct_strings n)"
   using unique_str_bij distinct_conv_nth by fastforce
+
+(* not sure how important those are *)
+
+lemma distinct_strings_prefix: "prefix (distinct_strings n) (distinct_strings (n+k))"
+  unfolding distinct_strings_def
+  apply (simp split: nat.splits)
+  using nat_upto_prefix map_mono_prefix by metis
+
+lemma distinct_strings_padded:
+  shows "distinct (map (pad k) (distinct_strings n))"
+proof -
+  let ?d = "distinct_strings n"
+  {
+    fix i j
+    assume a: "i < length ?d" "j < length ?d" "i \<noteq> j"
+    hence notin: "CHR ''_'' \<notin> set (?d ! i)" "CHR ''_'' \<notin> set (?d ! j)"
+      using distinct_strings_def unique_string_def notin_show_nat list_ball_nth by simp_all
+    from a have  "?d ! i \<noteq> ?d ! j" using distinct_strings_dist distinct_conv_nth by metis
+    hence "pad k (?d ! i) \<noteq> pad k (?d ! j)" using pad_neq notin by simp
+    hence "map (pad k) (distinct_strings n) ! i \<noteq> map (pad k) (distinct_strings n) ! j"
+      using a by auto
+  }
+  thus ?thesis using distinct_conv_nth by force
+qed
+
+section \<open> useless, ahem, legacy stuff \<close>
 
 
 definition distinctize :: "string list \<Rightarrow> string list \<Rightarrow> string list" where
